prescan.v
@@ -48,8 +48,9 @@ barrier(); // ϕspec
 // (iii) compaction if (flag[tid]) out[idx[tid]] = data[tid];
 *)
 
-Require Import GPUCSL.
+Require Import GPUCSL scan_lib.
 
+Section Prescan.
 Notation Tid := (Var 0).
 Notation In := (Var 1). 
 Notation Sum := (Var 2).
@@ -68,27 +69,323 @@ Infix "<C" := (Blt) (at level 70).
 Notation leftC ARR := (ARR +C Offset *C (Enum 2 *C Tid +C Enum 1) -C Enum 1).
 Notation rightC ARR := (ARR +C Offset *C (Enum 2 *C Tid +C Enum 2) -C Enum 1).
 
-Notation "E >>1" := (Ediv2 E) (at level 30).
+Notation Zn := Z.of_nat.
 
-Coercion Z.of_nat : nat >-> Z.
-Variable len : nat.
+Variable f_ini : nat -> Z.
+Variable ntrd : nat.
 
-Definition upsweep :=
-  Offset ::= 1 ;;
-  D ::= (len / 2) ;;
-  WhileI (FalseP) (0 <C D) (
+Hypothesis ntrd_is_p2 : exists e, ntrd = 2 ^ e.
+Lemma ntrd_neq_0 : ntrd <> 0.
+Proof.
+  destruct ntrd_is_p2; rewrite H; apply Nat.pow_nonzero; auto.
+Qed.
+
+Require Import Recdef.
+
+Function rdiv2 n {wf lt n} :=
+  match n with
+    | 0 => 0
+    | _ => if Nat.eq_dec (n mod 2) 0 then S (rdiv2 (n / 2)) else 0
+  end%nat.
+Proof.
+  intros; destruct Nat.eq_dec; try omega.
+  apply Nat.div_lt; omega.
+  apply lt_wf.
+Defined.
+
+Definition upInv (i : nat) :=
+  Ex (offset d : nat) (f : nat -> Z), 
+    !(Tid === Zn i) **
+    !(Offset === Zn offset) **
+    !(D === Zn d) **
+    !(pure ((d = 0) /\ (offset = ntrd * 2) \/ (d * offset = ntrd))) **
+    !(pure (forall i, f i = let m := min (2 ^ rdiv2 (i + 1)) offset in
+                      sum_of (i + 1 - m) m f_ini)) **
+    (if lt_dec i (ceil2 d) then is_array Sum (Nat.max 2 offset) f (i * (Nat.max 2 offset)) else emp).
+
+Definition bspec n :=
+  if Nat.eq_dec n 0 then
+    (MyVector.init (fun i : Fin.t ntrd => 
+       Ex (offset d : nat) (f : nat -> Z), 
+       !(Tid === Zn (nf i)) **
+       !(Offset === Zn offset) **
+       !(D === Zn d) **
+       !(pure ((d = 0) /\ (offset = ntrd * 2) \/ (d * offset = ntrd))) **
+       !(pure (forall i, f i = let m := min (2 ^ rdiv2 (i + 1)) offset in
+                               sum_of (i + 1 - m) m f_ini)) **
+       (if lt_dec (nf i) d then
+          is_array Sum (Nat.max 2 offset) f ((nf i) * (Nat.max 2 offset))
+        else emp)),
+     MyVector.init (fun i : Fin.t ntrd => 
+       Ex (offset d : nat) (f : nat -> Z), 
+       !(Tid === (Zn (nf i))) **
+       !(Offset === Zn offset) **
+       !(D === Zn d) **
+       !(pure ((d = 0) /\ (offset = ntrd * 2) \/ (d * offset = ntrd))) **
+       !(pure (forall i, f i = let m := min (2 ^ rdiv2 (i + 1)) offset in
+                               sum_of (i + 1 - m) m f_ini)) **
+       (if lt_dec (nf i) (ceil2 d) then is_array Sum (offset * 2) f ((nf i) * offset * 2) else emp)))
+  else default ntrd.
+
+Definition upsweep (i : nat) :=
+  Offset ::= 1%Z ;;
+  D ::= Zn ntrd ;;
+  WhileI (upInv i) (0%Z <C D) (
     Cbarrier 0 ;;
     Cif (Tid <C D) (
       Tmp1 ::= [leftC Sum] ;;
       Tmp2 ::= [rightC Sum] ;;
       [rightC Sum] ::= Tmp1 +C Tmp2
     ) (Cskip) ;;
-    Offset ::= Offset *C 2
+    Offset ::= Offset *C 2%Z ;;
+    D ::= D>>1
   ).
 
-Definition upInv (i : nat) : 
-  is_arrray Sum e 
+Ltac ex_dest_in H id :=
+  lazymatch type of H with
+    | ((Ex _, _) ** _) _ _ => apply ex_lift_l_in in H; destruct H as [id H]
+    | (_ ** (Ex _, _)) _ _ => apply ex_lift_r_in in H; destruct H as [id H]
+end.
 
+(* TODO: ex_lift_rに対応 *)
+Ltac sep_ex :=
+  lazymatch goal with
+    | [ |- ((Ex _, _) ** _) _ _] => apply ex_lift_l
+  end.
+
+Lemma fin_lt (n : nat) (i : Fin.t n) : (nf i) < n.
+Proof.
+  destruct (Fin.to_nat i); simpl; auto.
+Qed.
+
+Lemma is_array_unfold Arr len' f : forall s len,
+  len' < len ->
+  forall stc, 
+    stc ||= is_array Arr len f s <=>
+        is_array Arr len' f s **
+        (Arr +C (Zn (len' + s))%Z -->p (1, f (len' + s))) **
+        is_array Arr (len - len' - 1) f (S (len' + s)).
+Proof.
+  induction len'; intros s len Hlen stc.
+  - destruct len; try omega; simpl.
+    rewrite <-minus_n_O, emp_unit_l; reflexivity.
+  - destruct len; [inversion Hlen|]; simpl.
+    rewrite IHlen'; try omega.
+    rewrite <-plus_n_Sm; simpl; rewrite sep_assoc; autorewrite with sep. reflexivity.
+Qed.
+
+Hint Rewrite Nat2Z.inj_add Nat2Z.inj_mul Nat2Z.inj_sub : sep.
+Arguments div _ _ : simpl never.
+Arguments Nat.max _ _ : simpl never.
+
+Lemma div_pow2 : forall e n m, n * m = 2 ^ e -> exists e1 e2, n = 2 ^ e1 /\ m = 2 ^ e2.
+Proof.
+  induction e; intros n m Hnm.
+  - exists 0, 0; simpl.
+    apply mult_is_one; auto.
+  - rewrite pow_succ_r in Hnm; try omega.
+    assert (n mod 2 = 0 \/ n mod 2 = 1) by (pose proof (Nat.mod_upper_bound n 2); omega).
+    rewrite (Nat.div_mod n 2) in Hnm; auto; auto.
+    destruct H; rewrite H in Hnm.
+    + rewrite <-plus_n_O in Hnm.
+      rewrite <-mult_assoc, Nat.mul_cancel_l in Hnm; auto.
+      apply IHe in Hnm; try omega; destruct Hnm as (e1 & e2 & Hnm); exists (S e1), e2.
+      rewrite (Nat.div_mod n 2), H; auto; simpl. omega.
+    + assert (m mod 2 = 0 \/ m mod 2 = 1) by (pose proof (Nat.mod_upper_bound m 2); omega).
+      rewrite (Nat.div_mod m 2) in Hnm; auto; auto.
+      destruct H0; rewrite H0 in Hnm.
+      rewrite <-plus_n_O in Hnm.
+      rewrite <-mult_comm, <-mult_assoc, Nat.mul_cancel_l in Hnm; auto.
+      apply IHe in Hnm as (e1 & e2 & Hnm); exists e2, (S e1).
+      rewrite (Nat.div_mod m 2), (Nat.div_mod n 2), H, H0; simpl; omega.
+      ring_simplify in Hnm. 
+      cutrewrite (4 * (n / 2) * (m / 2) + 2 * (n / 2) + 2 * (m / 2) + 1 =
+                  2 * (2 * (n / 2) * (m / 2) + (n / 2) + (m / 2)) + 1) in Hnm; [omega|].
+      ring.
+Qed.
+
+Lemma rdiv2_mult (n m : nat) : m <> 0 -> 2 ^ n <= 2 ^ rdiv2 (2 ^ n * m).
+Proof.
+  intros Hm0; remember (2 ^ n * m) as nm eqn:eqnm; revert n m eqnm Hm0; functional induction (rdiv2 nm).
+  - intros; symmetry in eqnm; apply mult_is_O in eqnm; omega.
+  - intros n' m Hnm Hm0.
+    destruct n'; subst; [simpl; autorewrite with sep;
+                         pose proof (Nat.pow_nonzero 2 (rdiv2 (m / 2))); omega|].
+    rewrite !Nat.pow_succ_r', <-Nat.mul_le_mono_pos_l; auto.
+    eapply (IHn _ m); auto.
+    rewrite Nat.pow_succ_r'. 
+    cutrewrite (2 * 2 ^ n' * m = 2 ^ n' * m * 2); [|ring]; rewrite Nat.div_mul; auto.
+  - intros n' m Hnm Hm0.
+    destruct n'; auto; subst.
+    clear e0; rewrite Nat.pow_succ_r' in _x0. rewrite <-mult_assoc, mult_comm in _x0.
+    rewrite  Nat.mod_mul in _x0; omega.
+Qed.
+
+
+Lemma is_array_unfold' Arr len f : forall s,
+  0 < len ->
+  forall stc, 
+    stc ||= is_array Arr len f s <=>
+        is_array Arr (len - 1) f s **
+        (Arr +C (Zn (s + len - 1)) -->p (1, f (s + len - 1))).
+Proof.
+  induction len; intros s Hlen stc; try omega.
+  destruct len.
+  - simpl; rewrite <-plus_n_Sm, <-plus_n_O; simpl;
+    rewrite emp_unit_l, emp_unit_r, <-minus_n_O; reflexivity.
+  - remember (S len); simpl.
+    rewrite IHlen; try omega.
+    subst; simpl; rewrite <-!minus_n_O.
+    rewrite <-(plus_n_Sm s (S len)); simpl; rewrite <-minus_n_O, sep_assoc. reflexivity.
+Qed.
+
+Hint Resolve fin_lt.
+
+Lemma upsweep_correct (i : Fin.t ntrd) :
+  CSL bspec i 
+      (is_array Sum 1 f_ini (nf i))
+      (upsweep (nf i))
+      (if Nat.eq_dec (nf i) 0 then 
+         Ex f, 
+           !(pure (forall i, f i = let m := 2 ^ rdiv2 i in sum_of (i + 1 - m) m f)) ** 
+           is_array Sum (ntrd * 2) f 0
+       else emp).
+Proof.
+  pose proof ntrd_neq_0 as ntrd_neq_0.
+  unfold upsweep.
+  eapply rule_seq; [hoare_forward; intros ? ? [v H] | ].
+  { remember 1 in H. subA_normalize_in H. simpl in H. subst; exact H. }
+  eapply rule_seq; [hoare_forward; intros ? ? [v H] | ].
+  { remember 1 in H; subA_normalize_in H. simpl in H. subst. exact H. }
+  hoare_forward.
+  Hint Unfold bspec upInv.
+  
+  eapply rule_seq; [hoare_forward|].
+  { intros s h H.
+    ex_dest_in H offset; ex_dest_in H d; ex_dest_in H f.
+    sep_ex; exists offset; sep_ex; exists d; sep_ex; exists f.
+    sep_split_in H; sep_normal; sep_split; eauto.
+    change_in H.
+    { unfold_pures; unfold ceil2 in H; destruct Nat.eq_dec; try omega.
+      exact H. }
+    sep_rewrite_in_r emp_unit_r H. apply H. }
+
+  { autounfold; simpl; intros ? ? H; rewrite MyVector.init_spec in H. 
+    sep_rewrite_in emp_unit_r H. exact H. }
+  
+  repeat hoare_forward; revert x x0 x1; intros offset d fc.
+  eapply rule_seq. eapply rule_if_disj.
+  
+  { eapply Hbackward. 
+    Focus 2.
+    { intros s h H; sep_normal_in H; sep_split_in H.
+      change_in H.
+      { unfold_pures.
+        Lemma ceil2_leq (n : nat) : n <= ceil2 n.
+        Proof.
+          unfold ceil2; destruct Nat.eq_dec; omega.
+        Qed.
+        destruct lt_dec.
+        2: rewrite HP, HP1 in l; rewrite <-Nat2Z.inj_lt in l; pose proof (ceil2_leq d); omega.
+        assert (Hoff0 : offset <> 0) by (intros Hc; subst; destruct HP2; omega).
+        sep_rewrite_in is_array_unfold' H; try omega.
+        sep_rewrite_in is_array_unfold H. 
+        2: instantiate (1 := offset - 1); omega.
+        cutrewrite (offset - 1 + nf i * offset * 2 = offset * (2 * nf i + 1) - 1) in H.
+        Focus 2.
+        { cutrewrite (offset * (2 * nf i + 1) = nf i * offset * 2 + offset); [|ring]. 
+          generalize (nf i * offset * 2); intros; omega. } Unfocus.
+        cutrewrite (nf i * offset * 2 + offset * 2 - 1 = offset * (2 * nf i + 2) - 1) in H.
+        Focus 2.
+        { cutrewrite (offset * (2 * nf i + 2) = nf i * offset * 2 + offset * 2); [|ring].
+          omega. } Unfocus.
+
+        autorewrite with sep in H;
+          [|cutrewrite (1 = 1 * 1); [|auto]; apply Nat.mul_le_mono; omega..].
+        assert ((Sum +C (Zn offset * (Zn 2 * Zn (nf i) + Zn 1) - Zn 1)%Z ===
+                 Sum +C Zn offset *C (2 *C Zn (nf i) +C 1) -C 1) s emp_ph)%Z.
+        { unfold_conn; simpl. omega. }
+        sep_rewrite_in (mps_eq1) H; [|apply H0].
+        assert ((Sum +C (Zn offset * (Zn 2 * Zn (nf i) + Zn 2) - Zn 1)%Z ===
+                 Sum +C (Offset *C (2 *C Tid +C 2) -C 1)) s emp_ph)%Z.
+        { Arguments Z.mul _ _ : simpl never.
+          unfold_conn. simpl. congruence. }
+        sep_normal_in H. sep_lift_in H 3.
+        sep_rewrite_in (mps_eq1) H; [|apply H1].
+        exact H. }
+      (* Arguments Z.add _ _ : simpl never. *)
+      (* Arguments Z.mul _ _ : simpl never. *)
+      (* Arguments plus : simpl never. *)
+      (* Arguments mult : simpl never. *)
+      sep_combine_in H; exact H. } Unfocus.
+    eapply rule_seq; [hoare_forward; intros ? ? H; exact H |].
+    eapply rule_seq; [hoare_forward; intros ? ? H; exact H |].
+    hoare_forward; intros ? ? H; exact H. }
+
+  apply rule_skip.
+  eapply Hforward.
+  apply (rule_disj (Q1 := (upInv (nf i))) (Q2 := (upInv (nf i)))).  
+  3: intros s h [H1 | H2]; eauto.
+  eapply rule_seq; [hoare_forward; intros s h [v H]; subA_normalize_in H; ex_intro v H; simpl in H; exact H | ].
+  repeat hoare_forward.
+  intros s h [v H]; subA_normalize_in H. simpl in H; sep_split_in H.
+  unfold_pures; subst; autorewrite with sep in *.
+  exists (offset * 2), (d / 2).
+  exists (fun x => if Nat.eq_dec ((x + 1) mod (offset * 2)) 0 then
+                     (fc x + fc (x - offset)%nat)%Z
+                   else fc x).
+  sep_split; autorewrite with sep in *; eauto.
+  - unfold_conn; rewrite HP3 in *; rewrite <-Nat2Z.inj_lt in l. 
+    destruct HP6; try omega.
+    pose proof (Nat.div_mod d 2).
+    destruct ntrd_is_p2 as [e ntrd_2e]; rewrite ntrd_2e in H0; 
+    pose proof (div_pow2 _ _ _ H0) as (e1 & e2 & Hdo).
+    destruct e1; destruct Hdo; subst; [simpl; unfold div; simpl|].
+    left; split; eauto; simpl in H0; omega.
+    autorewrite with sep; auto.
+    rewrite pow_succ_r in H0; try omega; rewrite <-H0; right; ring.
+  - unfold_conn; intros ix.
+    destruct Nat.eq_dec; rewrite !HP7.
+    + assert (offset <> 0) by (destruct offset; destruct HP6; omega).
+      rewrite (Nat.div_mod (ix + 1) (offset * 2)), e; try omega; autorewrite with sep.
+    
+    
+      assert (exists e, offset = 2 ^ e) as [eoff Hoff].
+      { destruct HP6 as [[? ?]|?]; destruct ntrd_is_p2 as [? ?].
+        - subst; exists (S x); simpl; omega.
+        - subst. apply div_pow2 in H2; destruct H2 as [? [? [? ?]]]; eexists; eauto. }
+      assert ((ix + 1) / (2 ^ eoff * 2) <> 0).
+      { rewrite Nat.div_small_iff; try omega.
+        intros Hlt; rewrite Nat.mod_small in e; auto; omega. }
+      assert (exists k, ix + 1 = 2 ^ eoff * 2 * k /\ k <> 0) as [kix [Hix1 ?]].
+      { rewrite (Nat.div_mod (ix + 1) (2 ^ eoff * 2)); try omega; eexists; split.
+        subst; rewrite e, <-plus_n_O. reflexivity.
+        auto. }
+      subst. rewrite Nat.min_r.
+      2: rewrite <-mult_assoc; apply rdiv2_mult; omega.
+      assert (2 ^eoff <= ix).
+      { cutrewrite (ix = 2 ^ eoff * 2 * kix-1); [|omega].
+        rewrite (mult_comm _ 2); simpl; autorewrite with sep.
+        destruct kix; rewrite mult_comm; simpl; try omega.
+        generalize (2 ^ eoff) H0; intros; destruct n; simpl. omega.
+        generalize (kix * S (n + S n)); intros; omega. }
+      rewrite <-Nat.add_sub_swap; auto.
+      rewrite Hix1.
+      cutrewrite (2 ^ eoff * 2 * kix - 2 ^ eoff = 2 ^ eoff * (2 * kix - 1)); [|].
+      2: rewrite mult_minus_distr_l, mult_assoc, mult_1_r; auto.
+      rewrite Nat.min_r; [|apply rdiv2_mult; omega].
+      rewrite Nat.min_r; [|rewrite (mult_comm (2 ^ eoff) 2), <-Nat.pow_succ_r'; apply rdiv2_mult].
+      2: rewrite mult_comm, Nat.div_mul; auto.
+      rewrite (mult_comm (2 ^ eoff * 2) kix), Nat.div_mul; try omega.
+      cutrewrite (2 ^ eoff * (2 * kix - 1) - 2 ^ eoff = 2 ^ eoff * 2 * kix - 2 ^ eoff * 2).
+      2: rewrite mult_minus_distr_l, <-Nat.sub_add_distr; f_equal; ring.
+      cutrewrite (2 ^ eoff * 2 = 2 ^ eoff + 2 ^ eoff); [|omega].
+      rewrite sum_of_concat, Z.add_comm; f_equal.
+      f_equal. 
+      rewrite Nat.sub_add_distr, <-le_plus_minus; auto.
+      destruct kix; simpl; try omega; rewrite mult_comm; simpl. generalize (kix * (2 ^ eoff + 2 ^ eoff)); intros; omega.
+    + cutrewrite (min (2 ^ rdiv2 (ix + 1)) offset = min (2 ^ rdiv2 (ix + 1)) (offset * 2)); auto.
+      
 Definition downsweep :=
   D ::= 1 ;;
   WhileI (FalseP) (D <C len) (
